src/3d/Binding.fsti
@@ -44,3 +44,8 @@ val add_field_error_code_decls (ge: env)
   : ML (list decl)
 
 val initial_global_env (_:unit) : ML global_env
+
+val get_exported_decls (ge:global_env) (mname:string) : ML (list ident' & list ident')  //exported, private
+
+val finish_module (ge:global_env) (mname:string) (e_and_p:list ident' & list ident')
+  : ML global_env
